ActionSim.v
@@ -11,8 +11,8 @@ Set Implicit Arguments.
 Set Asymmetric Patterns.
 
 Section ActionSimAuto.
-  Context {t1 t2: Tree Elem}.
-  Variable rel: TreeState ElemState t1 -> TreeState ElemState t2 -> Prop.
+  Context {t1 t2: Tree DomainElem}.
+  Variable rel: TreeState DomainElemState t1 -> TreeState DomainElemState t2 -> Prop.
 
   Lemma LetAction_sim: forall {K K'} (s: string) (a1: Action type t1 K') (a2: Action type t2 K')
                               (cont1: type K' -> Action type t1 K) (cont2: type K' -> Action type t2 K),
@@ -56,8 +56,8 @@ Section ActionSimAuto.
 End ActionSimAuto.
 
 Section ActionSimAutoSameTree.
-  Context {t: Tree Elem}.
-  Variable rel: TreeState ElemState t -> TreeState ElemState t -> Prop.
+  Context {t: Tree DomainElem}.
+  Variable rel: TreeState DomainElemState t -> TreeState DomainElemState t -> Prop.
 
   Lemma ReadReg_sim: forall {K} (s: string) (x: RegPath t)
                            (cont1 cont2: _ -> Action type t K),
