Notations.v
@@ -102,108 +102,108 @@ End PurePathLookup.
 Arguments getLeafPath [A] t path.
 Arguments getChildLeafPath [A] t leafName.
 
-Definition getRegPath (t : Tree Elem) (path : string) : option (RegPath t) :=
+Definition getRegPath (t : Tree DomainElem) (path : string) : option (RegPath t) :=
   match getLeafPath t (splitDot path) as o return option (RegPath t) with
   | Some p =>
-      match isRegElem (getLeaf p) as b return (isRegElem (getLeaf p) = b) -> option (RegPath t) with
+      match isRegElem (getLeafElem p) as b return (isRegElem (getLeafElem p) = b) -> option (RegPath t) with
       | true => fun pf => Some {| regPath := p ; regPathPf := transparent_Is_true _ (Is_true_eq_left _ pf) |}
       | false => fun _ => None
       end eq_refl
   | None => None
   end.
 
-Definition getMemPath (t : Tree Elem) (path : string) : option (MemPath t) :=
+Definition getMemPath (t : Tree DomainElem) (path : string) : option (MemPath t) :=
   match getLeafPath t (splitDot path) as o return option (MemPath t) with
   | Some p =>
-      match isMemElem (getLeaf p) as b return (isMemElem (getLeaf p) = b) -> option (MemPath t) with
+      match isMemElem (getLeafElem p) as b return (isMemElem (getLeafElem p) = b) -> option (MemPath t) with
       | true => fun pf => Some {| memPath := p ; memPathPf := transparent_Is_true _ (Is_true_eq_left _ pf) |}
       | false => fun _ => None
       end eq_refl
   | None => None
   end.
 
-Definition getSendPath (t : Tree Elem) (path : string) : option (SendPath t) :=
+Definition getSendPath (t : Tree DomainElem) (path : string) : option (SendPath t) :=
   match getLeafPath t (splitDot path) as o return option (SendPath t) with
   | Some p =>
-      match isSendElem (getLeaf p) as b return (isSendElem (getLeaf p) = b) -> option (SendPath t) with
+      match isSendElem (getLeafElem p) as b return (isSendElem (getLeafElem p) = b) -> option (SendPath t) with
       | true => fun pf => Some {| sendPath := p ; sendPathPf := transparent_Is_true _ (Is_true_eq_left _ pf) |}
       | false => fun _ => None
       end eq_refl
   | None => None
   end.
 
-Definition getRecvPath (t : Tree Elem) (path : string) : option (RecvPath t) :=
+Definition getRecvPath (t : Tree DomainElem) (path : string) : option (RecvPath t) :=
   match getLeafPath t (splitDot path) as o return option (RecvPath t) with
   | Some p =>
-      match isRecvElem (getLeaf p) as b return (isRecvElem (getLeaf p) = b) -> option (RecvPath t) with
+      match isRecvElem (getLeafElem p) as b return (isRecvElem (getLeafElem p) = b) -> option (RecvPath t) with
       | true => fun pf => Some {| recvPath := p ; recvPathPf := transparent_Is_true _ (Is_true_eq_left _ pf) |}
       | false => fun _ => None
       end eq_refl
   | None => None
   end.
 
-Definition getRegPathTree (t : Tree Elem) (path : string) :=
+Definition getRegPathTree (t : Tree DomainElem) (path : string) :=
   forceOption (getRegPath t path).
 
-Definition getMemPathTree (t : Tree Elem) (path : string) :=
+Definition getMemPathTree (t : Tree DomainElem) (path : string) :=
   forceOption (getMemPath t path).
 
-Definition getSendPathTree (t : Tree Elem) (path : string) :=
+Definition getSendPathTree (t : Tree DomainElem) (path : string) :=
   forceOption (getSendPath t path).
 
-Definition getRecvPathTree (t : Tree Elem) (path : string) :=
+Definition getRecvPathTree (t : Tree DomainElem) (path : string) :=
   forceOption (getRecvPath t path).
 
-Definition getChildRegPath (t : Tree Elem) (name : string) : option (RegPath t) :=
+Definition getChildRegPath (t : Tree DomainElem) (name : string) : option (RegPath t) :=
   match getChildLeafPath t name as o return option (RegPath t) with
   | Some p =>
-      match isRegElem (getLeaf p) as b return (isRegElem (getLeaf p) = b) -> option (RegPath t) with
+      match isRegElem (getLeafElem p) as b return (isRegElem (getLeafElem p) = b) -> option (RegPath t) with
       | true => fun pf => Some {| regPath := p ; regPathPf := transparent_Is_true _ (Is_true_eq_left _ pf) |}
       | false => fun _ => None
       end eq_refl
   | None => None
   end.
 
-Definition getChildMemPath (t : Tree Elem) (name : string) : option (MemPath t) :=
+Definition getChildMemPath (t : Tree DomainElem) (name : string) : option (MemPath t) :=
   match getChildLeafPath t name as o return option (MemPath t) with
   | Some p =>
-      match isMemElem (getLeaf p) as b return (isMemElem (getLeaf p) = b) -> option (MemPath t) with
+      match isMemElem (getLeafElem p) as b return (isMemElem (getLeafElem p) = b) -> option (MemPath t) with
       | true => fun pf => Some {| memPath := p ; memPathPf := transparent_Is_true _ (Is_true_eq_left _ pf) |}
       | false => fun _ => None
       end eq_refl
   | None => None
   end.
 
-Definition getChildSendPath (t : Tree Elem) (name : string) : option (SendPath t) :=
+Definition getChildSendPath (t : Tree DomainElem) (name : string) : option (SendPath t) :=
   match getChildLeafPath t name as o return option (SendPath t) with
   | Some p =>
-      match isSendElem (getLeaf p) as b return (isSendElem (getLeaf p) = b) -> option (SendPath t) with
+      match isSendElem (getLeafElem p) as b return (isSendElem (getLeafElem p) = b) -> option (SendPath t) with
       | true => fun pf => Some {| sendPath := p ; sendPathPf := transparent_Is_true _ (Is_true_eq_left _ pf) |}
       | false => fun _ => None
       end eq_refl
   | None => None
   end.
 
-Definition getChildRecvPath (t : Tree Elem) (name : string) : option (RecvPath t) :=
+Definition getChildRecvPath (t : Tree DomainElem) (name : string) : option (RecvPath t) :=
   match getChildLeafPath t name as o return option (RecvPath t) with
   | Some p =>
-      match isRecvElem (getLeaf p) as b return (isRecvElem (getLeaf p) = b) -> option (RecvPath t) with
+      match isRecvElem (getLeafElem p) as b return (isRecvElem (getLeafElem p) = b) -> option (RecvPath t) with
       | true => fun pf => Some {| recvPath := p ; recvPathPf := transparent_Is_true _ (Is_true_eq_left _ pf) |}
       | false => fun _ => None
       end eq_refl
   | None => None
   end.
 
-Definition getChildRegPathTree (t : Tree Elem) (name : string) :=
+Definition getChildRegPathTree (t : Tree DomainElem) (name : string) :=
   forceOption (getChildRegPath t name).
 
-Definition getChildMemPathTree (t : Tree Elem) (name : string) :=
+Definition getChildMemPathTree (t : Tree DomainElem) (name : string) :=
   forceOption (getChildMemPath t name).
 
-Definition getChildSendPathTree (t : Tree Elem) (name : string) :=
+Definition getChildSendPathTree (t : Tree DomainElem) (name : string) :=
   forceOption (getChildSendPath t name).
 
-Definition getChildRecvPathTree (t : Tree Elem) (name : string) :=
+Definition getChildRecvPathTree (t : Tree DomainElem) (name : string) :=
   forceOption (getChildRecvPath t name).
 
 Declare Scope guru_scope.
@@ -241,23 +241,23 @@ Notation "u `! name" :=
 Notation "'UNION' ( ls , name ::= v )" :=
   (BuildUnion (ls := ls) (getFinStruct name%string ls) v) (at level 0, name at level 0, v at level 200): guru_scope.
 
-Definition readTreeReg {t} (s: TreeState ElemState t) (p: RegPath t) :
+Definition readTreeReg {t} (s: TreeState DomainElemState t) (p: RegPath t) :
   type (regKind (getRegFromPath p)) :=
   castStateReg p (readTreeState t s (regPath p)).
 Arguments readTreeReg [t] s p / .
 
-Definition readTreeMem {t} (s: TreeState ElemState t) (p: MemPath t) :
+Definition readTreeMem {t} (s: TreeState DomainElemState t) (p: MemPath t) :
   type (Array (getMemFromPath p).(memSize) (getMemFromPath p).(memKind)) **
   type (Array (getMemFromPath p).(memPort) (getMemFromPath p).(memKind)) :=
   castStateMem p (readTreeState t s (memPath p)).
 Arguments readTreeMem [t] s p / .
 
-Definition readTreeSend {t} (s: TreeState ElemState t) (p: SendPath t) :
+Definition readTreeSend {t} (s: TreeState DomainElemState t) (p: SendPath t) :
   list (type (getSendKind p)) :=
   castStateSend p (readTreeState t s (sendPath p)).
 Arguments readTreeSend [t] s p / .
 
-Definition readTreeRecv {t} (s: TreeState ElemState t) (p: RecvPath t) :
+Definition readTreeRecv {t} (s: TreeState DomainElemState t) (p: RecvPath t) :
   list (type (getRecvKind p)) :=
   castStateRecv p (readTreeState t s (recvPath p)).
 Arguments readTreeRecv [t] s p / .
